mext steps

Projects/Lindmar_Joost/BinaryHeapTree.lean
@@ -32,7 +32,7 @@ def extractMin: BinaryTree ENat → Option ENat
 | leaf => none
 | node _ v _ => some v
 
-def minHeap:  BinaryTree ENat → ENat
+def heapMin:  BinaryTree ENat → ENat
 | leaf => ⊤
 | node l v r => match l, r with
     | leaf, leaf => v
@@ -44,20 +44,16 @@ def minHeap:  BinaryTree ENat → ENat
                                     else
                                       if v <= rv then v
                                       else rv
--- def min:  BinaryTree ENat → ENat
--- | leaf => ⊤
--- | node l v r => if l
---     | leaf, leaf => v
---     | leaf, node _ rv _ => if v <= rv then v else rv
---     | node _ lv _, leaf => if v <= lv then v else lv
---     | node _ lv _, node _ rv _ =>  if lv <= rv then
---                                      if v <= lv then v
---                                      else lv
---                                     else
---                                       if v <= rv then v
---                                       else rv
 
-lemma extractMinCorrect (bt: BinaryTree ENat): isMinHeap bt → extractMin bt = minHeap bt := by sorry
+def enatMin (n m: ENat): ENat  := if n<=m then n else m
+
+def treeMin:  BinaryTree ENat → ENat
+| leaf => ⊤
+| node l v r => enatMin v (enatMin (treeMin l) (treeMin r))
+
+lemma extractMinCorrect (bt: BinaryTree ENat): isMinHeap bt → extractMin bt = treeMin bt := by sorry
+
+def isEmpty (bt: BinaryTree ENat):= bt = leaf
 
 def leftAndRightAreMinHeap: (BinaryTree ENat) →  Prop
 | leaf => true
@@ -105,12 +101,12 @@ all_goals simp
 
 
 
-lemma heapifyPreservesStructureAndRootMin (bt: BinaryTree ENat): (∃ l r v, bt = node l v r) →  ∃ l' v' r', heapify bt = node l' v' r' ∧ v' ≤ (minHeap bt) := by
+lemma heapifyPreservesStructureAndRootMin (bt: BinaryTree ENat): (∃ l r v, bt = node l v r) →  ∃ l' v' r', heapify bt = node l' v' r' ∧ v' ≤ (heapMin bt) := by
 intro hbt
 fun_induction heapify; all_goals expose_names
 . obtain ⟨l, r, v, hbt⟩ := hbt
   contradiction
-all_goals grind [minHeap]
+all_goals grind [heapMin]
 
 def contains: (BinaryTree ENat) → ENat → Prop
 | leaf, _ => false
@@ -128,36 +124,67 @@ fun_induction heapify generalizing v; all_goals try grind[contains]
 lemma containsIsNode (bt: BinaryTree ENat) (v: ENat): contains bt v → ∃ l v' r, bt = node l v' r := by
 fun_induction contains; all_goals simp
 
-lemma minHeapRootMin (bt l r: BinaryTree ENat) (v: ENat): bt = (node l v r) → isMinHeap bt → v = minHeap bt := by
+lemma minHeapRootMin (bt l r: BinaryTree ENat) (v: ENat): bt = (node l v r) → isMinHeap bt → v = heapMin bt := by
 intro hbt hmin
-fun_induction isMinHeap; all_goals grind [minHeap]
+fun_induction isMinHeap; all_goals grind [heapMin]
+
+lemma rootIsMinOfChildrenLeft (l r ll lr: BinaryTree ENat) (v lv: ENat): rootIsMinOfChildren (node l v r) →  l = (node ll lv lr) → v ≤ lv := by
+  intros; expose_names
+  rw [h_1] at h
+  cases r; all_goals grind[rootIsMinOfChildren]
 
 
-lemma minHeapMemberLeRoot (bt: BinaryTree ENat) (v: ENat):  isMinHeap bt →  contains bt v → v ≤ minHeap bt := by
+lemma rootIsMinOfChildrenRight (l r rl rr: BinaryTree ENat) (v rv: ENat): rootIsMinOfChildren (node l v r) →  r = (node rl rv rr) → v ≤ rv := by sorry
+
+lemma minHeapMemberLeRoot (bt: BinaryTree ENat) (v: ENat):  isMinHeap bt →  contains bt v →  heapMin bt ≤ v := by
 intro hmin hl
 fun_induction contains
 . contradiction
 . expose_names
-  cases hl
-  . sorry
-  sorry
-  -- cases hc; all_goals expose_names
-  -- . obtain ⟨v'', l', r', h⟩ := h
-  --   have: v_1 ≤ v := by grind
-  --   grind
-  -- . cases h; all_goals expose_names
-  --   . apply ih2
-  --     . apply minHeapThenLeftAndRightAreMinHeap at hmin
-  --       simp [leftAndRightAreMinHeap] at hmin
-  --       simp [hmin]
-  --     . sorry
-
-
---     . cases l
---       . contradiction
---       . expose_names
---         have: l = a.node a_1 a_2
-
+  cases hl; all_goals expose_names
+  . expose_names
+    rw [←h]
+    suffices v = (l.node v r).heapMin by grind
+    apply minHeapRootMin (l.node v r) l r v; all_goals grind
+  . cases h; all_goals expose_names
+    . have h2: l.contains v' := by exact h
+      apply containsIsNode at h2
+      obtain ⟨l'', v'', r'', h2 ⟩:= h2
+      have h3: l = l''.node v'' r'' := by exact h2
+      have hmin2: (l.node v r).isMinHeap := by assumption
+      have hmin3: (l.node v r).isMinHeap := by assumption
+      apply minHeapThenLeftAndRightAreMinHeap at hmin
+      simp [leftAndRightAreMinHeap] at hmin
+      have hlmin: l.isMinHeap := by grind
+      have hlmin2: l.isMinHeap := by grind
+      apply ih2 at hlmin
+      apply hlmin at h
+      grw[← h]
+      apply minHeapThenRootIsMinOfChildren at hmin2
+      apply rootIsMinOfChildrenLeft l r l'' r'' v v'' hmin2 at h2
+      have hhl: v'' = l.heapMin := by grind [minHeapRootMin]
+      have hh: v =(l.node v r).heapMin := by grind [minHeapRootMin]
+      grw [← hh, ← hhl]
+      exact h2
+    . have h2: r.contains v' := by exact h
+      apply containsIsNode at h2
+      obtain ⟨l'', v'', r'', h2 ⟩:= h2
+      have h3: r = l''.node v'' r'' := by exact h2
+      have hmin2: (l.node v r).isMinHeap := by assumption
+      have hmin3: (l.node v r).isMinHeap := by assumption
+      apply minHeapThenLeftAndRightAreMinHeap at hmin
+      simp [leftAndRightAreMinHeap] at hmin
+      have hlmin: r.isMinHeap := by grind
+      have hlmin2: r.isMinHeap := by grind
+      apply ih1 at hlmin
+      apply hlmin at h
+      grw[← h]
+      apply minHeapThenRootIsMinOfChildren at hmin2
+      apply rootIsMinOfChildrenRight l r l'' r'' v v'' hmin2 at h2
+      have hhl: v'' = r.heapMin := by grind [minHeapRootMin]
+      have hh: v =(l.node v r).heapMin := by grind [minHeapRootMin]
+      grw [← hh, ← hhl]
+      exact h2
 
 -- lemma heapifyEstablishesRootIsMinOfChildren (bt: BinaryTree ENat) (hbt: leftAndRightAreMinHeap bt): rootIsMinOfChildren (heapify bt) := by
 -- fun_induction heapify; all_goals expose_names; all_goals try grind[rootIsMinOfChildren, leftAndRightAreMinHeap]
@@ -203,23 +230,23 @@ lemma heapifyPreservesMinHeap (bt: BinaryTree ENat): isMinHeap bt → bt = heapi
 fun_induction heapify; all_goals expose_names; all_goals try grind
 . intro hbt
   by_contra
-  have hbtmin: v = minHeap (leaf.node v (rl.node rv rr)) := by grind [minHeapRootMin]
-  grind[minHeap]
+  have hbtmin: v = heapMin (leaf.node v (rl.node rv rr)) := by grind [minHeapRootMin]
+  grind[heapMin]
 . intro hbt
   by_contra
-  have hbtmin: v = minHeap ((ll.node lv lr).node v leaf) := by grind [minHeapRootMin]
-  grind[minHeap]
+  have hbtmin: v = heapMin ((ll.node lv lr).node v leaf) := by grind [minHeapRootMin]
+  grind[heapMin]
 . intro hbt
-  have hbtmin: v = minHeap ((ll.node lv lr).node v (rl.node rv rr)) := by grind [minHeapRootMin]
-  grind[minHeap]
+  have hbtmin: v = heapMin ((ll.node lv lr).node v (rl.node rv rr)) := by grind [minHeapRootMin]
+  grind[heapMin]
 . intro hbt
-  have hbtmin: v = minHeap ((ll.node lv lr).node v (rl.node rv rr)) := by grind [minHeapRootMin]
-  grind[minHeap]
+  have hbtmin: v = heapMin ((ll.node lv lr).node v (rl.node rv rr)) := by grind [minHeapRootMin]
+  grind[heapMin]
 
 lemma binTreeEq (l r l' r': BinaryTree ENat) (v v': ENat): (node l v r) = (node l' v' r') → r = r' := by
 grind only
 
-lemma decreaseRootIsHeap (l r: BinaryTree ENat) (v v': ENat): isMinHeap (node l v r) →  v' ≤ minHeap (node l v r) → isMinHeap (node l v' r) := by sorry
+-- lemma decreaseRootIsHeap (l r: BinaryTree ENat) (v v': ENat): isMinHeap (node l v r) →  v' ≤ minHeap (node l v r) → isMinHeap (node l v' r) := by sorry
 
 lemma heapifyEstablishesMinHeap' (bt l r: BinaryTree ENat) (v: ENat): bt = node l v r ∧  isMinHeap l ∧ isMinHeap r → isMinHeap (heapify bt) := by
 fun_induction heapify generalizing l r v; all_goals expose_names
@@ -227,7 +254,7 @@ fun_induction heapify generalizing l r v; all_goals expose_names
 . simp [isMinHeap]
 . intro ⟨hr, hminl, hminr⟩
   apply leftAndRightAreMinHeapAndRootIsMinOfChildrenToMinHeap
-  have: ∃ rl' v' rr', (rl.node v_1 rr).heapify = node rl' v' rr' ∧ v' ≤ minHeap (rl.node v_1 rr) := by
+  have: ∃ rl' v' rr', (rl.node v_1 rr).heapify = node rl' v' rr' ∧ v' ≤ heapMin (rl.node v_1 rr) := by
         apply heapifyPreservesStructureAndRootMin
         simp
   obtain ⟨rl', v', rr', hr1, hr2⟩ := this
@@ -247,13 +274,14 @@ fun_induction heapify generalizing l r v; all_goals expose_names
       apply ih1; all_goals grind
   . rw [hr1]
     simp [rootIsMinOfChildren]
-    have hrvmin : rv = minHeap (rl.node rv rr) := by sorry
+    have hrvmin : rv = heapMin (rl.node rv rr) := by sorry
     have hcontains: contains (rl.node rv rr) v' ∨ v'= v_1 := by sorry
     cases hcontains
     . expose_names
       apply minHeapMemberLeRoot r v' at hminr
       rw [← hrnode] at h_1
       apply hminr at h_1
+
       sorry
     . expose_names
       rw [h_1]
@@ -293,26 +321,6 @@ fun_induction heapify generalizing l r v; all_goals expose_names
 --   .
 
 lemma heapifyEstablishesMinHeap (bt: BinaryTree ENat): (hbt: leftAndRightAreMinHeap bt) → isMinHeap (heapify bt) := by
-fun_induction heapify; all_goals expose_names; all_goals try grind [isMinHeap]
-. intro hbt
-  simp [leftAndRightAreMinHeap] at hbt
-  obtain ⟨hb1, hb2⟩ := hbt
-  apply minHeapThenLeftAndRightAreMinHeap at hb2
-  apply ih1 at hb2
-  apply leftAndRightAreMinHeapAndRootIsMinOfChildrenToMinHeap
-  constructor
-  . simp [leftAndRightAreMinHeap]
-    constructor
-    . simp [isMinHeap]
-    . exact hb2
-  .
-    have: ∃ rl' v' rr', (rl.node v rr).heapify = node rl' v' rr' ∧ v' ≤ minHeap (rl.node v rr) := by
-      apply heapifyPreservesStructureAndRootMin
-      simp
-    obtain ⟨rl', v', rr', hr1, hr2⟩ := this
-    rw [hr1]
-
-    have: rv <= v' := by sorry
-
-    simp[rootIsMinOfChildren]
-    exact this
+cases bt
+. grind[isMinHeap,leftAndRightAreMinHeap, heapify]
+. grind[isMinHeap,leftAndRightAreMinHeap, heapifyEstablishesMinHeap']
